Low/Sel25519.v
@@ -22,6 +22,82 @@ Proof. intros; unfold list_cswap; destruct (Z.eqb b 0); go. Qed.
 Lemma list_cswap_Zlength_eq: forall b p q, Zlength p = Zlength q -> Zlength p = Zlength (list_cswap b p q).
 Proof. intros; unfold list_cswap; destruct (Z.eqb b 0); go. Qed.
 
+Lemma list_cswap_bound_le : forall p pmin pmax q qmin qmax,
+  Forall (fun x => pmin <= x <= pmax) p ->
+  Forall (fun x => qmin <= x <= qmax) q -> forall b,
+  Forall (fun x => Z.min pmin qmin <= x <= Z.max pmax qmax) (list_cswap b p q).
+Proof.
+move=> p pmin pmax q qmin qmax Hp Hq.
+elim => [|?|?]; unfold list_cswap ; simpl;
+eapply list.Forall_impl ; eauto;
+intros x H; simpl in H;
+destruct H as [Hmin Hmax]; split;
+eapply Z.le_trans ; eauto;
+try apply Z.le_min_l;try apply Z.le_min_r;try apply Z.le_max_l;try apply Z.le_max_r.
+Qed.
+
+Lemma list_cswap_bound_lt_le : forall p pmin pmax q qmin qmax,
+  Forall (fun x => pmin < x < pmax) p ->
+  Forall (fun x => qmin < x < qmax) q -> forall b,
+  Forall (fun x => Z.min pmin qmin <= x <= Z.max pmax qmax) (list_cswap b p q).
+Proof.
+move=> p pmin pmax q qmin qmax Hp Hq.
+elim => [|?|?]; unfold list_cswap ; simpl;
+eapply list.Forall_impl ; eauto;
+intros x H; simpl in H;
+destruct H as [Hmin Hmax]; split;apply Z.lt_le_incl;
+try solve[
+eapply Z.le_lt_trans ; eauto;
+try apply Z.le_min_l;try apply Z.le_min_r;try apply Z.le_max_l;try apply Z.le_max_r];
+eapply Z.lt_le_trans ; eauto;
+try apply Z.le_min_l;try apply Z.le_min_r;try apply Z.le_max_l;try apply Z.le_max_r.
+Qed.
+
+Lemma list_cswap_bound_lt : forall p pmin pmax q qmin qmax,
+  Forall (fun x => pmin < x < pmax) p ->
+  Forall (fun x => qmin < x < qmax) q -> forall b,
+  Forall (fun x => Z.min pmin qmin < x < Z.max pmax qmax) (list_cswap b p q).
+Proof.
+move=> p pmin pmax q qmin qmax Hp Hq.
+elim => [|?|?]; unfold list_cswap ; simpl;
+eapply list.Forall_impl ; eauto;
+intros x H; simpl in H;
+destruct H as [Hmin Hmax]; split;
+try solve[
+eapply Z.le_lt_trans ; eauto;
+try apply Z.le_min_l;try apply Z.le_min_r;try apply Z.le_max_l;try apply Z.le_max_r];
+eapply Z.lt_le_trans ; eauto;
+try apply Z.le_min_l;try apply Z.le_min_r;try apply Z.le_max_l;try apply Z.le_max_r.
+Qed.
+
 Close Scope Z.
 
 Definition Sel25519 b p q := list_cswap b p q.
+
+Lemma Sel25519_length_eq: forall b p q, length p = length q -> length p = length (Sel25519 b p q).
+Proof. rewrite /Sel25519 ; apply list_cswap_length_eq. Qed.
+
+Lemma Sel25519_Zlength_eq: forall b p q, Zlength p = Zlength q -> Zlength p = Zlength (list_cswap b p q).
+Proof. rewrite /Sel25519 ; apply list_cswap_Zlength_eq. Qed.
+
+Open Scope Z.
+
+Lemma Sel25519_bound_le : forall p pmin pmax q qmin qmax,
+  Forall (fun x => pmin <= x <= pmax) p ->
+  Forall (fun x => qmin <= x <= qmax) q -> forall b,
+  Forall (fun x => Z.min pmin qmin <= x <= Z.max pmax qmax) (list_cswap b p q).
+Proof. rewrite /Sel25519 ; apply list_cswap_bound_le. Qed.
+
+Lemma Sel25519_bound_lt_le : forall p pmin pmax q qmin qmax,
+  Forall (fun x => pmin < x < pmax) p ->
+  Forall (fun x => qmin < x < qmax) q -> forall b,
+  Forall (fun x => Z.min pmin qmin <= x <= Z.max pmax qmax) (Sel25519 b p q).
+Proof. rewrite /Sel25519 ; apply list_cswap_bound_lt_le. Qed.
+
+Lemma Sel25519_bound_lt : forall p pmin pmax q qmin qmax,
+  Forall (fun x => pmin < x < pmax) p ->
+  Forall (fun x => qmin < x < qmax) q -> forall b,
+  Forall (fun x => Z.min pmin qmin < x < Z.max pmax qmax) (Sel25519 b p q).
+Proof. rewrite /Sel25519 ; apply list_cswap_bound_lt. Qed.
+
+Close Scope Z.
